src/Utils/MapTreeN.v
@@ -1,0 +1,87 @@
+Require Import NArith.
+From coqutil Require Import Map.Interface.
+
+From Utils Require Import Base ExtraMaps.
+From Utils Require TrieMap.
+
+
+
+(* what I want (copied from MapTree): *)
+(*#[bypass_check(positivity)]*)
+Fail Inductive tree {key} {m : forall A, map.map key A} {A} :=
+| leaf : A -> tree
+| node : m tree -> tree
+(* a useful additional case: the all-inputs constant map.
+   Breaks extensionality when key is finite, but is important for generic join.
+ *)
+| top_node : tree -> tree.
+
+(* For eqsat purposes, we will always know statically the depth of the tree.
+   Thus, we can use a fixpoint on that depth as the type.
+ *)
+
+Section __.
+  Context {key} {m : forall A, map.map key A}.
+
+  Variant node (child : Type) :=
+    | fin_node : m child -> node child
+    | top_node : child -> node child.
+  Arguments fin_node {child}%type_scope _.
+  Arguments top_node {child}%type_scope _.
+
+  Section __.
+    Context (A : Type).
+    Fixpoint ntree n :=
+      match n with
+      | 0 => A
+      | S n => node (ntree n)
+      end.    
+  End __.
+
+  Section MapPlus.
+
+    Context `{@map_plus key m}.
+
+    
+    Section __.
+    Context {A B C : Type} (merge : A -> B -> C).
+    Definition merge_node (na : node A) (nb : node B) : node C :=
+      match na, nb with
+      | fin_node ma, fin_node mb => fin_node (map_intersect merge ma mb)
+      | top_node c1, top_node c2 => top_node (merge c1 c2)
+      | fin_node m, top_node c => fin_node (map_map (fun a => merge a c) m)
+      | top_node c, fin_node m => fin_node (map_map (merge c) m)
+      end.
+    End __.
+
+    Section __.
+    Context {A B C : Type} (merge : A -> B -> C).
+    
+    Fixpoint ntree_intersect n : ntree A n -> ntree B n -> ntree C n :=
+      match n with
+      | 0 => merge
+      | S n' => merge_node (ntree_intersect n')
+      end.
+    End __.
+
+    Section __.
+      Context {A B : Type}
+        (f : A -> B -> B).
+
+      (* Note: does not guarantee anything about order *)
+      Fixpoint map_tree_fold_values n : ntree A n -> B -> B :=
+        match n with
+        | 0 => f
+        | S n' =>
+            fun b =>
+              match b with
+              | fin_node m => map_fold_values (map_tree_fold_values n') m
+              | top_node c => map_tree_fold_values n' c
+              end
+        end.
+    End __.
+
+    
+  End MapPlus.
+  
+End __.
